vellvm_local/src/coq/Utils/InterpProp.v
@@ -591,7 +591,7 @@ Section interp_prop_extra.
     intros ? ? ?.
     pcofix self. pstep. intros u v ? euv. punfold euv.
     red in euv |- *. induction euv; pclearbot; eauto 7 with paco.
-    (*econstructor; eauto.
+    (* econstructor; eauto.
     intros. specialize (HK _ H2). pclearbot.
        right. eapply self; eauto. *)
   Qed.
